$$\begin{aligned}
&\sum_{i=0}^{+\infty}\sum_{j=i+1}^{+\infty}\left(\left\lfloor\dfrac{N}{p^i}\right\rfloor-\left\lfloor\dfrac{N}{p^{i+1}}\right\rfloor\right)\left(\left\lfloor\dfrac{N}{p^j}\right\rfloor-\left\lfloor\dfrac{N}{p^{j+1}}\right\rfloor\right)\left(j-i\right)\\
=&\sum_{i=0}^{+\infty}\left(\left\lfloor\dfrac{N}{p^i}\right\rfloor-\left\lfloor\dfrac{N}{p^{i+1}}\right\rfloor\right)\sum_{j=i+1}^{+\infty}\left(\left\lfloor\dfrac{N}{p^j}\right\rfloor-\left\lfloor\dfrac{N}{p^{j+1}}\right\rfloor\right)\left(j-i\right)\\
=&\sum_{i=0}^{+\infty}\left(\left\lfloor\dfrac{N}{p^i}\right\rfloor-\left\lfloor\dfrac{N}{p^{i+1}}\right\rfloor\right)\sum_{j=1}^{+\infty}\left(\left\lfloor\dfrac{N}{p^{i+j}}\right\rfloor-\left\lfloor\dfrac{N}{p^{i+j+1}}\right\rfloor\right)\cdot j\\
=&\sum_{i=0}^{+\infty}\left(\left\lfloor\dfrac{N}{p^i}\right\rfloor-\left\lfloor\dfrac{N}{p^{i+1}}\right\rfloor\right)\sum_{j=1}^{+\infty}\left\lfloor\dfrac{N}{p^{i+j}}\right\rfloor\\
=&\left(\sum_{i=0}^{+\infty}\left\lfloor\dfrac{N}{p^i}\right\rfloor\cdot\sum_{j=1}^{+\infty}\left\lfloor\dfrac{N}{p^{i+j}}\right\rfloor\right)-\left(\sum_{i=0}^{+\infty}\left\lfloor\dfrac{N}{p^{i+1}}\right\rfloor\cdot\sum_{j=1}^{+\infty}\left\lfloor\dfrac{N}{p^{i+j}}\right\rfloor\right)\\
=&N\cdot\sum_{j=1}^{+\infty}\left\lfloor\dfrac{N}{p^j}\right\rfloor+ \left(\sum_{i=1}^{+\infty}\left\lfloor\dfrac{N}{p^i}\right\rfloor\cdot\sum_{j=1}^{+\infty}\left\lfloor\dfrac{N}{p^{i+j}}\right\rfloor\right)-\left(\sum_{i=1}^{+\infty}\left\lfloor\dfrac{N}{p^{i}}\right\rfloor\cdot\sum_{j=1}^{+\infty}\left\lfloor\dfrac{N}{p^{i+j-1}}\right\rfloor\right)\\
=&N\cdot\sum_{j=1}^{+\infty}\left\lfloor\dfrac{N}{p^j}\right\rfloor+ \left(\sum_{i=1}^{+\infty}\left\lfloor\dfrac{N}{p^i}\right\rfloor\cdot\sum_{j=1}^{+\infty}\left(\left\lfloor\dfrac{N}{p^{i+j}}\right\rfloor-\left\lfloor\dfrac{N}{p^{i+j-1}}\right\rfloor\right)\right)\\
=&N\cdot\sum_{j=1}^{+\infty}\left\lfloor\dfrac{N}{p^j}\right\rfloor- \left(\sum_{i=1}^{+\infty}\left\lfloor\dfrac{N}{p^i}\right\rfloor\cdot\left\lfloor\dfrac{N}{p^i}\right\rfloor\right)\\
=&\sum_{i=1}^{+\infty}\left(N-\left\lfloor\dfrac{N}{p^i}\right\rfloor\right)\cdot\left\lfloor\dfrac{N}{p^i}\right\rfloor\\
\end{aligned}$$